Scott's work

src/tactic/refine_list.lean
@@ -2,38 +2,38 @@
 -- Released under Apache 2.0 license as described in the file LICENSE.
 -- Authors: Lucas Allen
 
- --To Do
-  -- * new examples which can't be solved with `library_search`
-  -- * Need another non misleading example for tactics.md
+-- TODO Documentation in tactics.md
 
 import tactic.library_search
 import data.mllist
 
+/-!
+TODO write a paragraph describing this file
+
+-/
+
 namespace tactic
 
---list_refine uses some functions from Library search
+--list_refine uses some functions from library_search
 open tactic.library_search
 
---get state function. Returns the current state
-meta def get_state : tactic tactic_state
-:= λ s, result.success s s
+/-- Returns the current tactic_state. -/
+meta def get_state : tactic tactic_state :=
+λ s, result.success s s
 
---set state function. Sets the current state to some state
-meta def set_state (s' : tactic_state) : tactic tactic_state
-:= λ s, result.success s s'
+/-- Sets the tactic_state. -/
+meta def set_state (s' : tactic_state) : tactic tactic_state :=
+λ s, result.success s s'
 
---Run and save state function. Slightly modified version of lock_tactic_state.
---This runs a tactic and returns a tuple of the result and it's tactic state.
+/-- Runs a tactic, returning the result and the new tactic_state, but then reverts the tactic_state. -/
+-- See also `lock_tactic_state`, which is similar but does not return the tactic_state.
 meta def run_and_save_state {α : Type} (t : tactic α) : tactic (α × tactic_state)
 | s := match t s with
        | result.success a s' := result.success (a, s') s
        | result.exception msg pos s' := result.exception msg pos s
 end
 
-meta def try_assumption_and_solve_by_elim : tactic unit :=
-try_core (any_goals (propositional_goal >> assumption)) >>
-  try_core (solve_by_elim { all_goals := tt }) >>
-  skip
+-- TODO finish converting to doc-strings
 
 --This function prints the apply tactic with the corresponding lemma/theorem with inputs
 meta def message (l : decl_data × tactic_state) (g : expr) : tactic string :=
@@ -44,50 +44,66 @@ do s ← get_state,
    return r
 
 --Runs through the list of things and prints a message for each one
-meta def print_messages (g : expr) : list (decl_data × tactic_state) → tactic string
-| []      := return ""
-| (l::ls) := do message l g >>= trace,
-                print_messages ls
+meta def print_messages (g : expr) (silent : bool) : list (decl_data × tactic_state) → tactic (list string)
+| []      := return []
+| (l::ls) := do r ← message l g,
+                if ¬ silent then trace r else skip,
+                rs ← print_messages ls,
+                return (r :: rs)
 
 meta def get_mldefs (defs : list decl_data) : mllist tactic decl_data :=
 mllist.of_list defs
 
+
+declare_trace silence_refine_list -- Turn off `exact ...` trace message
+declare_trace refine_list         -- Trace a list of all relevant lemmas
+
 --The main list_refine tactic, this is very similar to the main Library_search function
-meta def refine_list (num : ℕ := 50) : tactic string :=
+meta def refine_list (num : ℕ := 50) (discharger : tactic unit := done) : tactic (list string) :=
 do (g::gs) ← get_goals,
    t ← infer_type g,
 
+   -- Make sure that `solve_by_elim` doesn't just solve the goal immediately:
+   (do
+       r ← lock_tactic_state (solve_by_elim { discharger := discharger } >> tactic_statement g),
+       when (¬ is_trace_enabled_for `silence_refine_list) $ tactic.trace r,
+       return $ [to_string r]) <|>
+   -- Otherwise, let's actually try applying library lemmas.
+   (do
    -- Collect all definitions with the correct head symbol
    defs ← library_defs (head_symbol t),
    -- Sort by length; people like short proofs
    let defs := defs.qsort(λ d₁ d₂, d₁.l ≤ d₂.l),
+   when (is_trace_enabled_for `refine_list) $ (do
+     trace format!"Found {defs.length} relevant lemmas:",
+     trace $ defs.map (λ ⟨d, n, m, l⟩, (n, m.to_string))),
    -- Turn defs into an mllist
    let mldefs := get_mldefs defs,
    -- Filter out the lemmas that cannot be used with refine
    let results := mldefs.mfilter_map
-     (λ d, run_and_save_state ((apply_declaration try_assumption_and_solve_by_elim d) >> pure d)),
+     (λ d, run_and_save_state ((apply_declaration ff discharger d) >> pure d)),
+   -- PROJECT it would be better to sort not just by `num_goals`, but by the pair
+   -- `(num_goals, -num_hyps_used)`, where `num_hyps_used` is a putative function that
+   -- counts numbers of appearances of local hypotheses in `result`.
    let results_with_num_goals := results.mmap
         (λ d, lock_tactic_state $ do set_state d.2, ng ← num_goals, return (d, ng)),
    -- Get the first num elements of the successful lemmas
    L ← results_with_num_goals.take num,
    let L := L.qsort(λ d₁ d₂, d₁.2 ≤ d₂.2),
-   -- Print the fist num successful lemmas
+   -- Print the first num successful lemmas
    if L.length = 0 then do
-    let r := "There are no applicable lemmas or theorems",
-    trace r,
-    return r
+    fail "There are no applicable lemmas or theorems"
    else
-   if (¬ is_trace_enabled_for `silence_library_search)
-   then print_messages g (L.map (λ d, d.1))
-   else return ""
+    print_messages g (is_trace_enabled_for `silence_refine_list) (L.map (λ d, d.1)))
 
 end tactic
 
 namespace interactive
 /--
-`refine_list` is a modification of `library_search`, which lists possible usages of the `refine`
+`refine_list` lists possible usages of the `refine`
 tactic and leaves the tactic state unchanged. It is intended as a complement of the search
 function in your editor, the `#find` tactic, and `library_search`.
+
 `refine_list` takes an optional natural number `num` as input and returns the first `num`
 (or less, if all possibilities are exhausted) possibilities ordered by length of lemma names.
 The default for `num` is `50`.
@@ -98,3 +114,6 @@ For performance reasons `refine_list` uses monadic lazy lists (`mllist`). This m
 meta def refine_list := tactic.refine_list
 
 end interactive
+
+#doc_blame
+#sanity_check
