test/refine_list.lean
@@ -5,18 +5,16 @@
 import tactic.refine_list
 
 /- Turn off trace messages so they don't pollute the test build: -/
---set_option trace.silence_library_search true
+set_option trace.silence_refine_list true
 
 open tactic
 
 --refine_list fails if there are no goals.
-
 example : true :=
 begin
   trivial,
   success_if_fail { refine_list },
 end
-
 
 example (a : Prop) : a ∨ true :=
 begin
@@ -27,7 +25,6 @@ example {a a' : ℕ} (h : a == a') : a = a' :=
 begin
   refine_list, exact eq_of_heq h,
 end
-
 example {a b c : ℤ} (h₁ : a = b) (h₂ : b = c) : a = c :=
 begin
   refine_list, exact eq.trans h₁ h₂,
@@ -38,9 +35,34 @@ begin
   refine_list, exact rfl,
 end
 
-example (n : nat) : n + 2 > n :=
+example (n : nat) : n < n + 1 :=
 begin
   refine_list,
+  exact nat.lt.base n
+end
+example (n : nat) : n < n + 2 :=
+begin
+  refine_list,
+  refine nat.lt.step _, -- this wasn't the first result; humans still necessary :-(
+  refine_list,
+  exact nat.lt.base n
 end
 
-open nat
+example (a b : Prop) : (a ∨ true) ∧ (b ∨ true) :=
+begin
+  refine_list,
+  refine ⟨_, _⟩, -- wasn't the first result, because it created two new goals
+  refine_list,
+  exact or.inr trivial,
+  refine_list,
+  exact or.inr trivial,
+end
+
+example (A B : Prop) (a : A) (b : unit → B) : A ∧ B :=
+begin
+  refine_list,
+  refine ⟨a, _⟩,
+  replace b := b (),
+  refine_list,
+  exact b,
+end
